cancellation/ElimRel.v
@@ -4,12 +4,28 @@ Require Import SModCancel HModInline.
 
 Section REL.
   Context `{Σ: GRA.t}.
-  Variable ginv: Sk.t -> invspec.
-  Variable stb: Sk.t -> gname -> option fspec.
   Variable md: SMod.t.
-  Notation iProp := (iProp Σ).
-  Let sk: Sk.t := SMod.sk md.
 
+  Definition stb_global: Sk.t -> gname -> option fspec :=
+    fun sk fn =>
+      option_map (fun scfsp => scfsp.2.(fsb_fspec))
+        (alist_find fn (SMod.modsem md sk).(SModSem.fnsems)).
+
+  Lemma stb_in_alist_find
+        (sk: Sk.t) fn fsp
+        (SKINCL: incl (SMod.sk md) sk) 
+        (SKWF: Sk.wf sk)
+        (SOME: stb_global sk fn = Some fsp)
+      :
+      exists l fbody, 
+        alist_find fn (SModSem.fnsems (SMod.modsem md sk))
+        = Some (l, {|fsb_fspec :=fsp; fsb_body := fbody|}).
+  Proof.
+    unfold stb_global in *.
+    destruct (alist_find fn _) eqn: FIND; ss.
+    inv SOME. destruct p. destruct f. s. eauto.
+  Qed.
+  
   Definition hmod_elim_head X P : Any.t -> itree hmodE ((nat * X * nat * X) * Any.t)
     :=
     fun varg =>
@@ -32,18 +48,18 @@ Section REL.
       trigger (Assume (Q my_tid x vret ret));;; tau;;
       Ret vret.
       
-  Definition HoareYieldE ginv' (tid: nat) : itree hmodE unit :=
-    trigger (Guarantee (ginv' tid));;; tau;;
+  Definition HoareYieldE ginv (tid: nat) : itree hmodE unit :=
+    trigger (Guarantee (ginv tid));;; tau;;
     trigger (Yield tid);;; tau;;
     my_tid <- trigger Tid;; tau;;
-    trigger (Assume (ginv' my_tid)).
+    trigger (Assume (ginv my_tid)).
 
-  Definition HoareSpawnE ginv' (fsp: fspec) (fn: gname) (varg: Any.t) : itree hmodE nat :=
+  Definition HoareSpawnE ginv (fsp: fspec) (fn: gname) (varg: Any.t) : itree hmodE nat :=
     x <- trigger (Choose fsp.(meta));; tau;;
     arg <- trigger (Choose Any.t);; tau;;
     tid <- trigger (Spawn fn arg);; tau;;
-    trigger (Guarantee (ginv' tid -∗ fsp.(precond) tid x varg arg));;; tau;;
-    HoareYieldE ginv' tid;;; 
+    trigger (Guarantee (ginv tid -∗ fsp.(precond) tid x varg arg));;; tau;;
+    HoareYieldE ginv tid;;; 
     Ret tid.
 
   Definition SpawnCancelE (fn: gname) (varg: Any.t) : itree hmodE nat :=
@@ -51,7 +67,7 @@ Section REL.
     trigger (Yield tid);;;
     Ret tid.
 
-  Variant elim_rel_def {sk0 A}
+  Variant elim_rel_def {ginv sk A}
     (self: list (nat * {X: Type & X}) -> itree hmodE A -> itree hmodE A -> Prop)
     : list (nat * {X: Type & X}) -> itree hmodE A -> itree hmodE A -> Prop
   :=
@@ -109,29 +125,29 @@ Section REL.
         (x <- @hmod_elim_tail X Q (tid, m, tid, m) vret;; tau;; ktrT x)
 
   | elim_rel_spawn l f fn args ktrS ktrT
-      (STB: stb sk0 fn = Some f)
+      (STB: stb_global sk fn = Some f)
       (KTR: forall x, self l (ktrS x) (ktrT x))
     :
     elim_rel_def self l (SpawnCancelE fn args >>= ktrS)
-                        (x <- HoareSpawnE (ginv sk0) f fn args;; ktrT x)
+                        (x <- HoareSpawnE (ginv sk) f fn args;; ktrT x)
 
   | elim_rel_yield tid l ktrS ktrT
       (KTR: forall x, self l (ktrS x) (ktrT x))
     :
     elim_rel_def self l (trigger (Yield tid) >>= ktrS)
-                        (x <- HoareYieldE (ginv sk0) tid;; ktrT x)
+                        (x <- HoareYieldE (ginv sk) tid;; ktrT x)
   .
 
-  Definition elim_rel {sk0 A} :=
-    paco3 (@elim_rel_def sk0 A) bot3.
+  Definition elim_rel {ginv sk A} :=
+    paco3 (@elim_rel_def ginv sk A) bot3.
 
-  Definition thread_local_rel {sk0} itrS itrT : Prop :=
-    @elim_rel sk0 Any.t [] itrS itrT.
+  Definition thread_local_rel {ginv sk} itrS itrT : Prop :=
+    @elim_rel ginv sk Any.t [] itrS itrT.
 
-  Lemma elim_rel_def_mon {sk0 A} r1 r2
+  Lemma elim_rel_def_mon {ginv sk A} r1 r2
     (REL: r1 <3= r2)
   :
-  @elim_rel_def sk0 A r1 <3= @elim_rel_def sk0 A r2.
+  @elim_rel_def ginv sk A r1 <3= @elim_rel_def ginv sk A r2.
   Proof.
     i. destruct PR; eauto using @elim_rel_def.
   Qed.
@@ -157,8 +173,8 @@ Section REL.
     ii. destruct IN; econs; eauto.
   Qed.
 
-  Lemma elim_rel_bindC_spec {sk0 A}:
-    elim_rel_bindC <4= gupaco3 (@elim_rel_def sk0 A) (cpn3 (@elim_rel_def sk0 A)).
+  Lemma elim_rel_bindC_spec {ginv sk A}:
+    elim_rel_bindC <4= gupaco3 (@elim_rel_def ginv sk A) (cpn3 (@elim_rel_def ginv sk A)).
   Proof.
     Local Opaque hmod_elim_tail.
     eapply wrespect3_uclo; eauto with paco.
@@ -184,54 +200,14 @@ End REL.
 Hint Resolve cpn3_wcompat: paco.
 Hint Resolve elim_rel_def_mon: paco.
 
-
 Section CANCEL.
   Context `{Σ: GRA.t}.
-  Variable ginv: Sk.t -> invspec.
-  Variable stb: Sk.t -> gname -> option fspec.
   Variable md: SMod.t.
-  Notation iProp := (iProp Σ).
-  Let sk: Sk.t := SMod.sk md.
-  Let ms (sk0: Sk.t) (SKINCL: incl sk sk0) (SKWF: Sk.wf sk0) := 
-    SMod.modsem md sk0.
-  Let sbtb (sk0: Sk.t) (SKINCL: incl sk sk0) (SKWF: Sk.wf sk0): alist gname (list string * fspecbody) := 
-    (ms sk0 SKINCL SKWF).(SModSem.fnsems).
-  Let _stb (sk0: Sk.t) (SKINCL: incl sk sk0) (SKWF: Sk.wf sk0): alist gname (list string * fspec) := 
-    List.map (map_snd (fun '(fn, fs) => (fn, fs.(fsb_fspec)))) (sbtb sk0 SKINCL SKWF).
-
-  Hypothesis STBCOMPLETE:
-    forall 
-      sk0 (SKINCL: incl sk sk0) (SKWF: Sk.wf sk0)
-      fn scfsp (FIND: alist_find fn (_stb sk0 SKINCL SKWF) = Some scfsp), stb sk0 fn = Some scfsp.2.
-  Hypothesis STBSOUND:
-    forall 
-      sk0 (SKINCL: incl sk sk0) (SKWF: Sk.wf sk0)
-      fn (FIND: alist_find fn (_stb sk0 SKINCL SKWF) = None),
-      (<<NONE: stb sk0 fn = None>>).
-
-  Lemma stb_in_alist_find
-        (sk0: Sk.t) fn fsp
-        (SKINCL: incl sk sk0) 
-        (SKWF: Sk.wf sk0)
-        (SOME: stb sk0 fn = Some fsp)
-      :
-        exists l fbody, 
-          alist_find fn (SModSem.fnsems (SMod.modsem md sk0)) = Some (l, {|fsb_fspec :=fsp; fsb_body := fbody|}).
-  Proof.
-    destruct (alist_find fn (_stb sk0 SKINCL SKWF)) eqn: FIND; cycle 1.
-    { eapply STBSOUND in FIND. des. clarify. }
-    unfold _stb, sbtb, ms in FIND.
-    rewrite alist_find_map_snd/o_map in FIND. des_ifs.
-    destruct p0, f. exists l, fsb_body. repeat f_equal.
-    assert (alist_find fn (_stb sk0 SKINCL SKWF) = Some (l, fsb_fspec)).
-    { rewrite/_stb alist_find_map_snd /o_map /sbtb /ms Heq. ss. }
-    eapply STBCOMPLETE in H. ss. rewrite SOME in H. inv H. ss.
-  Qed.
 
   Lemma HoareYield_sandbox
-      scopes ginv' tid
+      scopes ginv tid
     :
-    HModSem.sandbox scopes (HoareYield ginv' tid) = HoareYield ginv' tid.
+    HModSem.sandbox scopes (HoareYield ginv tid) = HoareYield ginv tid.
   Proof.
     unfold HoareYield.
     rewrite HModSB.transl_bind HModSB.transl_ag. f_equal. extensionalities.
@@ -241,11 +217,11 @@ Section CANCEL.
   Qed. 
 
   Lemma HoareYield_hpI
-      prog ginv' tid ktr
+      prog ginv tid ktr
     :
-    inline_hp prog (HoareYield ginv' tid >>= ktr)
+    inline_hp prog (HoareYield ginv tid >>= ktr)
     =
-    x <- HoareYieldE ginv' tid;; tau;; inline_hp prog (ktr x).
+    x <- HoareYieldE ginv tid;; tau;; inline_hp prog (ktr x).
   Proof. 
     unfold HoareYield, HoareYieldE. ired.
     rewrite HIRed.bind_ag. f_equal. extensionalities. ired. do 2 f_equal.
@@ -255,9 +231,9 @@ Section CANCEL.
   Qed.
 
   Lemma HoareSpawn_sandbox
-      scopes ginv' f fn args
+      scopes ginv f fn args
     :
-    HModSem.sandbox scopes (HoareSpawn ginv' f fn args) = HoareSpawn ginv' f fn args.
+    HModSem.sandbox scopes (HoareSpawn ginv f fn args) = HoareSpawn ginv f fn args.
   Proof.
     unfold HoareSpawn.
     rewrite HModSB.transl_bind HModSB.transl_core. f_equal. extensionalities.
@@ -269,11 +245,11 @@ Section CANCEL.
   Qed. 
 
   Lemma HoareSpawn_hpI
-      prog ginv' f fn args ktr
+      prog ginv f fn args ktr
     :
-    inline_hp prog (HoareSpawn ginv' f fn args >>= ktr)
+    inline_hp prog (HoareSpawn ginv f fn args >>= ktr)
     =
-    x <- HoareSpawnE ginv' f fn args;; tau;; inline_hp prog (ktr x).
+    x <- HoareSpawnE ginv f fn args;; tau;; inline_hp prog (ktr x).
   Proof.
     unfold HoareSpawn, HoareSpawnE. ired.
     rewrite HIRed.bind_core. f_equal. extensionalities. ired. do 2 f_equal.
@@ -307,10 +283,10 @@ Section CANCEL.
   Qed.
 
   Lemma HoareCall_inline_cancel
-      sk0 scopes fn varg scp fsp fbody 
-      (FIND: alist_find fn (SModSem.fnsems (SMod.modsem md sk0)) = Some (scp, {|fsb_fspec := fsp; fsb_body := fbody|}))
+    ginv sk scopes fn varg scp fsp fbody 
+    (FIND: alist_find fn (SModSem.fnsems (SMod.modsem md sk)) = Some (scp, {|fsb_fspec := fsp; fsb_body := fbody|}))
     :
-    inline_hp (prog (SModSem.to_hmod (ginv sk0) (stb sk0) (SMod.modsem md sk0))) (HModSem.sandbox scopes (HoareCall fsp fn varg))
+    inline_hp (prog (SModSem.to_hmod (ginv sk) (stb_global md sk) (SMod.modsem md sk))) (HModSem.sandbox scopes (HoareCall fsp fn varg))
     =
     (* head *)
     my_tid <- trigger Tid;; tau;;
@@ -322,8 +298,8 @@ Section CANCEL.
     varg' <- trigger (Take Any.t);; tau;;
     trigger (Assume (precond fsp my_tid' m' varg' arg));;; tau;; 
     (* body *)
-    vret' <- inline_hp (prog (SModSem.to_hmod (ginv sk0) (stb sk0) (SMod.modsem md sk0))) 
-                       (HModSem.sandbox scp (interp_smod (ginv sk0) (stb sk0) (fbody varg')));;
+    vret' <- inline_hp (prog (SModSem.to_hmod (ginv sk) (stb_global md sk) (SMod.modsem md sk))) 
+                       (HModSem.sandbox scp (interp_smod (ginv sk) (stb_global md sk) (fbody varg')));;
     (* tail *)
     ret <- trigger (Choose Any.t);; tau;;
     trigger (Guarantee (postcond fsp my_tid' m' vret' ret));;; tau;; tau;; tau;;
@@ -370,16 +346,16 @@ Section CANCEL.
   Qed.
 
   Lemma HoareCall_inline
-      sk0 scopes fn varg scp fsp fbody 
-      (FIND: alist_find fn (SModSem.fnsems (SMod.modsem md sk0)) = Some (scp, {|fsb_fspec := fsp; fsb_body := fbody|}))
+    ginv sk scopes fn varg scp fsp fbody 
+    (FIND: alist_find fn (SModSem.fnsems (SMod.modsem md sk)) = Some (scp, {|fsb_fspec := fsp; fsb_body := fbody|}))
     :
-    inline_hp (prog (SModSem.to_hmod (ginv sk0) (stb sk0) (SMod.modsem md sk0))) (HModSem.sandbox scopes (HoareCall fsp fn varg))
+    inline_hp (prog (SModSem.to_hmod (ginv sk) (stb_global md sk) (SMod.modsem md sk))) (HModSem.sandbox scopes (HoareCall fsp fn varg))
     =
     (* head *)
     '((my_tid, x, my_tid', x'), varg'):_ <- (hmod_elim_head (meta fsp) (precond fsp) varg);;
     (* body *)
-    vret' <- inline_hp (prog (SModSem.to_hmod (ginv sk0) (stb sk0) (SMod.modsem md sk0))) 
-                       (HModSem.sandbox scp (interp_smod (ginv sk0) (stb sk0) (fbody varg')));;
+    vret' <- inline_hp (prog (SModSem.to_hmod (ginv sk) (stb_global md sk) (SMod.modsem md sk))) 
+                       (HModSem.sandbox scp (interp_smod (ginv sk) (stb_global md sk) (fbody varg')));;
     (* tail *)
     hmod_elim_tail (meta fsp) (postcond fsp) (my_tid, x, my_tid', x') vret'. 
   Proof.
@@ -389,23 +365,23 @@ Section CANCEL.
   Qed.
 
   Definition elim_head_body 
-    sk0 scp fsp fbody varg
+    ginv sk scp fsp fbody varg
     :=
     ('((my_tid, x, my_tid', x'), varg'):_ <- (hmod_elim_head (meta fsp) (precond fsp) varg);;
     (* body *)
-    vret' <- inline_hp (prog (SModSem.to_hmod (ginv sk0) (stb sk0) (SMod.modsem md sk0))) 
-                       (HModSem.sandbox scp (interp_smod (ginv sk0) (stb sk0) (fbody varg')));;
+    vret' <- inline_hp (prog (SModSem.to_hmod (ginv sk) (stb_global md sk) (SMod.modsem md sk))) 
+                       (HModSem.sandbox scp (interp_smod (ginv sk) (stb_global md sk) (fbody varg')));;
     Ret ((my_tid, x, my_tid', x'), vret')).
 
   Lemma HoareCall_inline2
-      sk0 scopes fn varg scp fsp fbody 
-      (FIND: alist_find fn (SModSem.fnsems (SMod.modsem md sk0)) = Some (scp, {|fsb_fspec := fsp; fsb_body := fbody|}))
+    ginv sk scopes fn varg scp fsp fbody 
+    (FIND: alist_find fn (SModSem.fnsems (SMod.modsem md sk)) = Some (scp, {|fsb_fspec := fsp; fsb_body := fbody|}))
     :
-    inline_hp (prog (SModSem.to_hmod (ginv sk0) (stb sk0) (SMod.modsem md sk0))) 
-        (HModSem.sandbox scopes (HoareCall fsp fn varg))
+    inline_hp (prog (SModSem.to_hmod (ginv sk) (stb_global md sk) (SMod.modsem md sk))) 
+      (HModSem.sandbox scopes (HoareCall fsp fn varg))
     =
     (* head *)
-    RET <- elim_head_body sk0 scp fsp fbody varg;;
+    RET <- elim_head_body ginv sk scp fsp fbody varg;;
     (* tail *)
     (fun RET =>
       let '((my_tid, x, my_tid', x'), vret') := RET in
@@ -429,15 +405,15 @@ Section CANCEL.
       end; try unfold IT at 2.
 
   Lemma elim_rel_refl
-      sk0 scopes itr
-      (SKINCL: incl sk sk0)
-      (SKWF: Sk.wf sk0)
+      ginv sk scopes itr
+      (SKINCL: incl (SMod.sk md) sk)
+      (SKWF: Sk.wf sk)
     :
-    @elim_rel _ ginv stb sk0 _ []
-      (inline_hp (prog (SModSemCancel.to_hmod (SMod.modsem md sk0))) 
+    @elim_rel _ md ginv sk _ []
+      (inline_hp (prog (SModSemCancel.to_hmod (SMod.modsem md sk))) 
           (HModSem.sandbox scopes (interp_smod_cancel itr)))
-      (inline_hp (prog (SModSem.to_hmod (ginv sk0) (stb sk0) (SMod.modsem md sk0))) 
-          (HModSem.sandbox scopes (interp_smod (ginv sk0) (stb sk0) itr))).
+      (inline_hp (prog (SModSem.to_hmod (ginv sk) (stb_global md sk) (SMod.modsem md sk))) 
+          (HModSem.sandbox scopes (interp_smod (ginv sk) (stb_global md sk) itr))).
   Proof. 
     unfold elim_rel.
     ginit. revert itr scopes. gcofix CIH. i.
@@ -456,7 +432,7 @@ Section CANCEL.
       gstep. econs. gstep. econs. eauto with paco.
     - rewrite SModRed.interp_bind SModRed.interp_sch SCancelRed.bind SCancelRed.sch. ired. 
       unfold handle_schE_hmodE, handle_schE_hmodE_cancel. depdes s.
-      + destruct (stb sk0 fn) eqn:STB; ired; cycle 1.
+      + destruct (stb_global md sk fn) eqn:STB; ired; cycle 1.
         { 
           unfold triggerNB. ired. 
           rewrite !HModSB.transl_bind HModSB.transl_core. ired. 
@@ -479,7 +455,7 @@ Section CANCEL.
         gstep. econs. gstep. econs. eauto with paco.
     - rewrite SModRed.interp_bind SModRed.interp_call SCancelRed.bind SCancelRed.call.
       unfold handle_callE_hmodE. depdes c. 
-      destruct (stb sk0 fn) eqn: STB; ired; cycle 1.
+      destruct (stb_global md sk fn) eqn: STB; ired; cycle 1.
       { 
         unfold triggerNB. 
         rewrite !HModSB.transl_bind HModSB.transl_core. ired. 
@@ -489,8 +465,8 @@ Section CANCEL.
       rewrite HModSB.transl_call HIRed.call HIRed.bind.
       
       assert (FIND := stb_in_alist_find).
-      specialize (FIND sk0 fn f SKINCL SKWF STB). des.
-      destruct (alist_find fn (List.map (map_snd (λ ksb : list string * fspecbody, (ksb.1, interp_sb_hp_cancel ksb.2))) (SModSem.fnsems (SMod.modsem md sk0)))) eqn: FINDS; cycle 1.
+      specialize (FIND md sk fn f SKINCL SKWF STB). des.
+      destruct (alist_find fn (List.map (map_snd (λ ksb : list string * fspecbody, (ksb.1, interp_sb_hp_cancel ksb.2))) (SModSem.fnsems (SMod.modsem md sk)))) eqn: FINDS; cycle 1.
       { exfalso. rewrite alist_find_map_snd FIND in FINDS. clarify.  }
       ired. rewrite FINDS. destruct p. rewrite alist_find_map_snd FIND in FINDS. s in FINDS. inv FINDS. 
       ired. unfold HModSem.sandbox_body. s. 
@@ -498,7 +474,7 @@ Section CANCEL.
       eassert (ITREE = tau;; x <- (a <- inline_hp _ (HModSem.sandbox l0 (x <- _ args;; tau;; Ret x));; tau;; Ret a);; tau;; _).
       {
         unfold ITREE. do 2 f_equal. 
-        instantiate (3:= prog (SModSemCancel.to_hmod (SMod.modsem md sk0))).
+        instantiate (3:= prog (SModSemCancel.to_hmod (SMod.modsem md sk))).
         ired. rewrite HModSB.transl_bind HIRed.bind. ired. f_equal.  
         extensionalities. rewrite HModSB.transl_tau !HIRed.tau. ired.
         do 4 f_equal.
@@ -509,13 +485,10 @@ Section CANCEL.
       eassert (ITREE0 = x <- (a <- inline_hp _ _;; tau;; Ret a);; tau;; _ x).
       {
         instantiate (2:= HModSem.sandbox scopes (HoareCall f fn args)).
-        instantiate (2:= prog (SModSem.to_hmod (ginv sk0) (stb sk0) (SMod.modsem md sk0))).
+        instantiate (2:= prog (SModSem.to_hmod (ginv sk) (stb_global md sk) (SMod.modsem md sk))).
         rewrite /ITREE0 !HIRed.bind. ired. f_equal.
         extensionalities. ired. rewrite HModSB.transl_tau HIRed.tau.
-        repeat f_equal. 
-        instantiate (1:= fun x => inline_hp (prog (SModSem.to_hmod (ginv sk0) (stb sk0) (SMod.modsem md sk0))) 
-        (HModSem.sandbox scopes (interp_smod (ginv sk0) (stb sk0) (ktrH' x)))).
-        s. refl.
+        instantiate (1:= fun H0 => _ (_ (_ (_ H0)))). refl.
       }
       rewrite H H0. clear ITREE ITREE0 H H0.
 
@@ -526,7 +499,7 @@ Section CANCEL.
         rewrite HModSB.transl_bind HIRed.bind.
         set (inline_hp _ _ ). eassert (i = _ args).
         { unfold i. instantiate (1:= fun x => inline_hp _ (_ (_ x))). refl. }
-        remember (λ x : Any.t, inline_hp (prog (SModSemCancel.to_hmod (SMod.modsem md sk0))) (HModSem.sandbox l0 (_ x))).
+        remember (λ x : Any.t, inline_hp (prog (SModSemCancel.to_hmod (SMod.modsem md sk))) (HModSem.sandbox l0 (_ x))).
         rewrite H. clear i H.
         ired. gstep. econs. 
         { 
