cancellation/CancelHead.v
@@ -1,0 +1,73 @@
+Require Import Common.
+Require Import SMod2HMod HMod2Mod Mod2ITree SMod HMod Mod Skeleton.
+Require Import SimGlobal.
+Require Import SModCancel HModInline ElimRel StRed CancelLib.
+
+Section CANCEL.
+  Context `{Σ: GRA.t}.
+  Variable md: SMod.t.
+
+  Import CancelTAC.
+
+  Lemma cancel_aux_head
+    ginv sk (SKINCL: incl (SMod.sk md) sk) (SKWF: Sk.wf sk) r ps pt srcs tgts
+    cid st (rs rt rs0 rt0: Σ) l X X0 (meta: X) P Q ktrS ktrT varg
+    (WFS: ✓ rs) (WFT: ✓ rt)
+    (UPD: Own rs ==∗ Own rt)
+    (LENS: cid < List.length srcs)
+    (LENT: cid < List.length tgts)
+    (LEN: List.length srcs = Datatypes.length tgts)
+    (RET: ∀ vret ret : Any.t, cid = 0 → Q cid meta vret ret ⊢ ⌜vret = ret⌝)
+    (RELS: ∀ k x y, cid ≠ k → srcs !! k = Some x → tgts !! k = Some y → thread_rel md ginv sk cid k x y)
+    (KTR: ∀ tid (m: X0) varg, upaco3 (@elim_rel_def _ md ginv sk _) bot3 ((tid, existT X0 m) :: l) (ktrS varg) (ktrT (tid, m, tid, m, varg)))
+    (SRC : srcs !! cid = Some (Ret ();;; interp_hp (tau;; ktrS varg)))
+    (TGT : tgts !! cid = Some (Ret ();;; interp_hp (cancel_term md ginv sk cid meta Q (x <- hmod_elim_head X0 P varg;; ktrT x))))
+    (CIH: ∀ rs rt srcs tgts cid st ps pt X (meta : X) Q itrS itrT l,
+        ✓ rs → (Own rs ==∗ Own rt) →
+        List.length srcs = List.length tgts →
+        cid < List.length srcs → cid < List.length tgts → 
+        srcs !! cid = Some (Ret ();;; interp_hp itrS) →
+        tgts !! cid = Some (Ret ();;; interp_hp (cancel_term md ginv sk cid meta Q itrT)) →
+        (∀ vret ret, cid = 0 → Q cid meta vret ret ⊢ ⌜vret = ret⌝) →
+        paco3 (@elim_rel_def _ md ginv sk _) bot3 l itrS itrT →
+        (∀ k x y, cid ≠ k → srcs !! k = Some x → tgts !! k = Some y → thread_rel md ginv sk cid k x y)
+        → CANCEL_GOAL md r ginv sk rs0 rt0 ps pt srcs tgts cid st rs rt)
+    :
+    CANCEL_GOAL md (gpaco7 _simg (cpn7 _simg) bot7 r) ginv sk rs0 rt0 ps pt srcs tgts cid st rs rt.
+  Proof.
+    r. _iter. _iter. rewrite SRC TGT. ired.
+    hide_r. tau 2.
+    reveal ITREE. hide_l. tau 1.
+    iterT 2. iterL. _coreA. ls.
+    iterT 2. iterL. _coreA. ls.
+    iterT 2. iterL. _supd.
+    iterL. _coreA. iterL. _coreA. ls.
+    iterL. _supd. iterL. _supd.
+    iterT 3. iterL. ls. tau 1.
+    iterT 2. iterL. _coreE x. ls.
+    iterT 2. iterL. _coreE varg. ls.
+    iterT 2.
+    hexploit (Own_bupd_split rt); eauto.
+    i. des.
+    iterL. _coreE a1. ls.
+    iterL. _supd.
+    assert (UPD': Own rs ==∗ Own (a1 ⋅ x1)).
+    {
+      iIntros "H". iPoseProof (UPD with "H") as ">H".
+      iPoseProof (H with "H") as ">[H0 H1]".
+      iPoseProof (H1 with "H1") as "H1".
+      iModIntro. rewrite Own_op. iFrame.
+    }
+    assert (VALID: ✓ (a1 ⋅ x1)).
+    { eapply Own_wand_valid with (a1 := rs); eauto. }
+    iterL. _coreE VALID. ls.
+    iterL. _coreE H0. ls.
+    iterL. _supd. iterL. _supd.
+    iterT 2.
+    reveal ITREE.
+    done_by_CIH CIH LKX LKY.
+    i. rewrite !list_lookup_insert_ne in H3, H4; eauto.
+  Qed.
+
+End CANCEL.
+
