cancellation/CancelSpawn.v
@@ -1,0 +1,172 @@
+Require Import Common.
+Require Import SMod2HMod HMod2Mod Mod2ITree SMod HMod Mod Skeleton.
+Require Import SimGlobal.
+Require Import SModCancel HModInline ElimRel StRed CancelLib.
+
+Section CANCEL.
+  Context `{Σ: GRA.t}.
+  Variable md: SMod.t.
+
+  Import CancelTAC.
+
+  Lemma cancel_aux_spawn
+    ginv sk (SKINCL: incl (SMod.sk md) sk) (SKWF: Sk.wf sk) r ps pt srcs tgts
+    cid st (rs rt rs0 rt0: Σ) l X (meta: X) Q ktrS ktrT f fn args
+    (WFS: ✓ rs) (WFT: ✓ rt)
+    (UPD: Own rs ==∗ Own rt)
+    (LENS: cid < List.length srcs)
+    (LENT: cid < List.length tgts)
+    (LEN: List.length srcs = Datatypes.length tgts)
+    (RET: ∀ vret ret : Any.t, cid = 0 → Q cid meta vret ret ⊢ ⌜vret = ret⌝)
+    (RELS: ∀ k x y, cid ≠ k → srcs !! k = Some x → tgts !! k = Some y → thread_rel md ginv sk cid k x y)
+    (STB: stb_global md sk fn = Some f)
+    (KTR: ∀ tid, upaco3 (@elim_rel_def _ md ginv sk _) bot3 l (ktrS tid) (ktrT tid))
+    (SRC : srcs !! cid = Some (Ret ();;; interp_hp (x <- SpawnCancelE fn args;; ktrS x)))
+    (TGT : tgts !! cid = Some (Ret ();;; interp_hp (cancel_term md ginv sk cid meta Q (x <- HoareSpawnE (ginv sk) f fn args;; ktrT x))))
+    (CIH: ∀ rs rt srcs tgts cid st ps pt X (meta : X) Q itrS itrT l,
+        ✓ rs → (Own rs ==∗ Own rt) →
+        List.length srcs = List.length tgts →
+        cid < List.length srcs → cid < List.length tgts → 
+        srcs !! cid = Some (Ret ();;; interp_hp itrS) →
+        tgts !! cid = Some (Ret ();;; interp_hp (cancel_term md ginv sk cid meta Q itrT)) →
+        (∀ vret ret, cid = 0 → Q cid meta vret ret ⊢ ⌜vret = ret⌝) →
+        paco3 (@elim_rel_def _ md ginv sk _) bot3 l itrS itrT →
+        (∀ k x y, cid ≠ k → srcs !! k = Some x → tgts !! k = Some y → thread_rel md ginv sk cid k x y)
+        → CANCEL_GOAL md r ginv sk rs0 rt0 ps pt srcs tgts cid st rs rt)
+    :
+    CANCEL_GOAL md (gpaco7 _simg (cpn7 _simg) bot7 r) ginv sk rs0 rt0 ps pt srcs tgts cid st rs rt.
+  Proof.
+    r. _iter. _iter. rewrite SRC TGT. ired.
+    hide_l. _coreA.
+    iterT 2. iterL. _coreA. ls.
+    iterT 2. iterL. tau 1. ls.
+    rewrite !length_insert.
+    rewrite <- insert_app_l; eauto.
+    match goal with [|-context[tgts ++ ?t]] =>
+      assert(LTT: cid < List.length (tgts ++ t)) by (rewrite length_app; nia)
+    end.
+    iterT 2. iterL. _supd.
+    iterL. _coreA. ls. iterL. _coreA. ls.
+    iterL. _supd. iterL. _supd.
+    iterT 2. iterL. _supd.
+    iterL. _coreA. ls. iterL. _coreA. ls.
+    iterL. _supd. iterL. _supd.
+    iterT 2. iterL. tau 1. ls.
+    reveal ITREE.
+    hide_r. tau 1.
+    rewrite -insert_app_l; eauto.
+    match goal with [|-context[srcs ++ ?t]] =>
+      assert(LTS: cid < List.length (srcs ++ t)) by (rewrite length_app; nia)
+    end.
+    iterT 2.
+    iterL. tau 1. ls.
+    hexploit stb_in_alist_find; eauto. i. des.
+    reveal ITREE.
+    rewrite !alist_find_map_snd !H. s.
+    erewrite wrap_elimI_well_scoped; cycle 1.
+    {
+      instantiate (1:= fn).
+      s. unfold interp_sb_hp_cancel. s.
+      rewrite alist_find_map_snd H. ss.
+    }
+    erewrite wrap_elimI_well_scoped; cycle 1.
+    {
+      instantiate (1:= fn).
+      s. unfold interp_sb_hp. s.
+      rewrite alist_find_map_snd H. ss.
+    }
+    ired.
+    unfold interp_hp_fun, inline_hp_fun, HModSem.sandbox_body. s.
+    unfold interp_sb_hp, interp_sb_hp_cancel. s.
+    hide_l. _iter.
+    rewrite list_lookup_insert_ne; try nia.
+    rewrite list_lookup_length. ired. tau 1.
+    assert (forall x, List.length tgts < List.length (tgts ++ [x])).
+    { i. rewrite length_app. s. nia. }
+    hexploit (Own_bupd_split rt); eauto. i. des.
+    hexploit (Own_bupd_split x1); eauto.
+    {
+      hexploit (Own_wand_valid rt (a1 ⋅ x1)); eauto.
+      {
+        iIntros "H". iPoseProof (H1 with "H") as ">[H0 H1]".
+        iPoseProof (H3 with "H1") as "H1".
+        iModIntro. rewrite Own_op. iFrame.
+      }
+      i. eapply cmra_valid_op_r. eauto.
+    }
+    i. des.
+    iterT 2. iterL. _coreE x. ls.
+    iterT 2. iterL. _coreE args. ls.
+    iterT 2. iterL. _coreE (a0 ⋅ a1). ls. iterL. _supd.
+    assert (UPD': Own rs ==∗ Own (a0 ⋅ a1 ⋅ x3)).
+    {
+      iIntros "H". iPoseProof (UPD with "H") as ">H".
+      iPoseProof (H1 with "H") as ">[H0 H1]".
+      iPoseProof (H3 with "H1") as "H1".
+      iPoseProof (H4 with "H1") as ">[H1 H2]".
+      iPoseProof (H6 with "H2") as "H2".
+      iModIntro. rewrite !Own_op. iFrame.
+    }
+    assert (VALID: ✓(a0 ⋅ a1 ⋅ x3)).
+    { eapply Own_wand_valid with (a1 := rs); eauto. }
+    iterL. _coreE VALID. ls.
+    assert (SAT: Own (a0 ⋅ a1) ⊢ precond f (base.length tgts) x args x0).
+    {
+      iIntros "[H0 H1]".
+      iPoseProof (H5 with "H0") as "H0".
+      iPoseProof (H2 with "H1") as "H1".
+      iApply "H1". eauto.
+    }
+    iterL. _coreE SAT. ls.
+    iterL. _supd. iterL. _supd.
+    iterT 2.
+    reveal ITREE.
+    rewrite LEN.
+    prb. gbase. pclearbot.
+    eapply CIH; try (rewrite !length_insert !length_app; s; nia); swap 4 6; swap 5 6.
+    { auto. }
+    { auto. }
+    {
+      rewrite list_lookup_insert_ne; try nia.
+      rewrite -LEN list_lookup_length bind_ret_l. refl.
+    }
+    { eapply elim_rel_refl; eauto. }
+    {
+      rewrite list_lookup_insert; eauto; cycle 1.
+      { rewrite length_insert length_app. s. nia. }
+      grind. unfold cancel_term, inline_hp.
+      match goal with [|-context[translate (_ ?scopes) ?itr]]=>
+        fold (HModSem.sandbox scopes itr)
+      end.
+      rewrite -HIRed.iter_handle_bind HModSB.transl_bind.
+      do 4 f_equal. extensionalities.
+      rewrite HModSB.transl_bind HModSB.transl_core.
+      f_equal. extensionalities.
+      rewrite HModSB.transl_bind HModSB.transl_ag HModSB.transl_ret.
+      refl.
+    }
+    { i. nia. }
+    i. rewrite list_lookup_insert_ne in H9; eauto.
+    destruct (Nat.eq_dec cid k).
+    {
+      subst k. rewrite list_lookup_insert in H9; cycle 1.
+      { rewrite length_app. s. nia. }
+      rewrite list_lookup_insert in H8; cycle 1.
+      { rewrite length_app. s. nia. }
+      inv H9. econs; eauto; cycle 1.
+      { destruct (Nat.eq_dec cid (base.length tgts)); try nia. grind. }
+      {
+        destruct (Nat.eq_dec cid (base.length tgts)); try nia.
+        instantiate (1:= ktrT (base.length tgts)).
+        unfold yield_post. ired. rewrite -interp_hp_tau.
+        do 6 f_equal. extensionalities. grind.
+      }
+      eapply KTR.
+    }
+    rewrite !list_lookup_insert_ne in H8, H9; try nia.
+    eapply lookup_snoc_Some in H8, H9. des; try nia.
+    specialize (RELS k x5 y n H11 H10).
+    inv RELS. econs; eauto; des_ifs.
+  Qed.
+
+End CANCEL.
