common/CRIS.v
@@ -4,6 +4,7 @@ Require Export Skeleton STB.
 Require Export SMod HMod PMod.
 Require Export ISim ITactics.
 Require Export CtxRefine CtxRefineFacts MainAdequacy.
+Require Export Cancellation.
 
 From iris.algebra Require Export auth excl excl_auth functions frac agree gmap big_op.
 From stdpp Require Export coPset namespaces.
